Translation.v
@@ -67,30 +67,35 @@ Section TransDef.
   Inductive exp_trans : S.context -> S.exp -> S.type -> E.mode -> E.context ->
     E.loc_mode -> E.exp -> E.type -> Prop :=
   | TRnat : forall sG n p md eG d,
+      S.exp_wt sG (S.Enat n) (S.Typ S.Tnat p) ->
       exp_trans sG (S.Enat n) (S.Typ S.Tnat p)
                 md eG d (E.Enat n) (E.Typ E.Tnat p)
   | TRvar : forall sG x t t' eG md d,
+      S.exp_wt sG (S.Evar x) t ->
       ttrans t d t' ->
       E.var_context eG x = Some t' ->
       exp_trans sG (S.Evar x) t
                 md eG d (E.Evar x) t'
   | TRcnd : forall sG cnd p d md md' eG,
+      S.exp_wt sG (S.Eloc (Cnd cnd)) (S.Typ S.Tcond p) ->
       d (Cnd cnd) = md' ->
       exp_trans sG (S.Eloc (Cnd cnd)) (S.Typ S.Tcond p)
                 md eG d (E.Eloc (Cnd cnd)) (E.Typ (E.Tcond md') p)
   | TRisunset : forall sG cnd md' md eG d p,
+      S.exp_wt sG (S.Eisunset cnd) (S.Typ S.Tnat p) ->
       d (Cnd cnd) = md' ->
       md' = E.Normal \/ md = md' ->
       exp_trans sG (S.Eisunset cnd) (S.Typ S.Tnat p)
                 md eG d (E.Eisunset cnd) (E.Typ E.Tnat p)
   | TRloc : forall sG l t rt (q: sec_level) t' md' md eG d q,
+      S.exp_wt sG (S.Eloc (Not_cnd l)) (S.Typ (S.Tref t rt) q) ->
       ttrans (S.Typ (S.Tref t rt) q) d (E.Typ (E.Tref t' md' rt) q) ->
       E.loc_context eG (Not_cnd l) = Some (t', rt) ->
       d (Not_cnd l) = md' ->
       exp_trans sG (S.Eloc (Not_cnd l)) (S.Typ (S.Tref t rt) q)
                 md eG d (E.Eloc (Not_cnd l)) (E.Typ (E.Tref t' md' rt) q)
   | TRderef : forall sG (eG: E.context) e s p s' q md eG d e' md' rt,
-      (* S.exp_wt sG e (S.Typ (S.Tref (S.Typ s p) rt) q) -> *)
+      S.exp_wt sG (S.Ederef e) (S.Typ s (JoinP p q)) ->
       exp_trans sG e (S.Typ (S.Tref (S.Typ s p) rt) q)
                 md eG d e' (E.Typ (E.Tref (E.Typ s' p) md' rt) q) ->
       md' = E.Normal \/ md = md' ->
@@ -98,6 +103,7 @@ Section TransDef.
                 md eG d (E.Ederef e')
                 (E.Typ s' (JoinP p q))
   | TRop : forall sG op e1 s p s' md eG d e1' e2 q e2',
+      S.exp_wt sG (S.Ebinop e1 e2 op) (S.Typ s (JoinP p q)) ->
       exp_trans sG e1 (S.Typ s p) md eG d e1' (E.Typ s' p) ->
       exp_trans sG e2 (S.Typ s q) md eG d e2' (E.Typ s' q) ->
       exp_trans sG (S.Ebinop e1 e2 op)
@@ -119,20 +125,24 @@ Section TransDef.
                    E.loc_mode -> E.com -> E.context -> set E.enclave ->
                    Prop :=
   | TRskip : forall pc sG eG U md K d,
+      S.com_wt pc sG U S.Cskip sG ->     
       context_trans sG d eG ->
       E.mode_alive md K ->
       com_trans pc sG U S.Cskip sG
                 md eG K d E.Cskip eG K
   | TRassign : forall pc sG sG' U x e e' md eG K d eG' q s s',
+      S.com_wt pc sG U (S.Cassign x e) sG' ->
       context_trans sG d eG ->
       exp_trans sG e (S.Typ s q) md eG d e' (E.Typ s' q) ->
       policy_le (JoinP pc q) (liftp (LevelP L)) \/ md <> E.Normal ->
       E.mode_alive md K ->
-      (* XXX sG' and eG' *)
+      eG' = E.Cntxt (update (E.var_context eG) x (Some (E.Typ s' (JoinP pc q))))
+                    (E.loc_context eG) ->
+      sG' = S.Cntxt (update (S.var_context sG) x (Some (S.Typ s (JoinP pc q))))
+                    (S.loc_context sG) ->
       com_trans pc sG U (S.Cassign x e) sG'
                 md eG K d (E.Cassign x e') eG' K
       
-
   with prog_trans : policy -> S.context -> set condition -> S.prog ->
                     S.context -> E.mode -> E.context -> set E.enclave ->
                     E.loc_mode -> E.com -> E.context -> set E.enclave ->
@@ -145,7 +155,7 @@ Section TransDef.
 End TransDef.
 
 Section TransLemmas.
-  Hint Constructors btrans ttrans context_trans. (*
+  Hint Constructors btrans ttrans context_trans.
   Lemma trans_exp_ttrans : forall sG e t md eG d e' t',
       exp_trans sG e t md eG d e' t' ->
       ttrans t d t'.
@@ -160,7 +170,7 @@ Section TransLemmas.
       btrans s d s'.
   Proof.
     intros. apply trans_exp_ttrans in H. now inversion H.
-  Qed.*)
+  Qed.
 End TransLemmas.
 
 Section TransProof.
@@ -175,34 +185,30 @@ Section TransProof.
   Admitted.
   
   Lemma exp_trans_sound : forall e sG t md eG d e' t',
-      S.exp_wt sG e t ->
       exp_trans sG e t md eG d e' t' ->
       E.exp_type md eG d e' t'.
   Proof.
     intros.
-    induction H0.
-    - inversion H. eapply E.ETnat.
-    - now eapply E.ETvar.
-    - inversion H. now eapply E.ETcnd.
-    - inversion H. eapply E.ETunset with (md':=md'); intuition.
-    - inversion H. now eapply E.ETloc.
-    - inversion H. subst.
-      eapply E.ETderef with (md':=md') (rt:=rt); intuition.
-    - inversion H. subst. apply trans_exp_btrans in H0_.
-      inversion H0_. subst. eapply E.ETbinop; auto.
-    - inversion H. subst. eapply E.ETlambda.
-      now eapply prog_trans_sound with (sGp:=sGp) (c:=c) (sGm:=sGm).
-  Admitted.
+    induction H; inversion H; subst; try constructor; auto.
+    - eapply E.ETunset; intuition.
+    - eapply E.ETderef with (md':=md') (rt:=rt); intuition.
+    - apply trans_exp_btrans in H0. inversion H0. subst. now constructor.
+    - now eapply prog_trans_sound with (sGp:=sGp) (c:=c) (sGm:=sGm).
+  Qed.
 
-  Check S.com_wt.
   Lemma com_trans_sound : forall pc sG U c sG' md eG K d c' eG' K',
-      S.com_wt pc sG U c sG' ->
       com_trans pc sG U c sG' md eG K d c' eG' K' ->
       E.com_type pc md eG K U d c' eG' K'.
   Proof.
-    intros. induction H0.
+    intros. induction H.
     - now constructor.
-    - inversion H. subst. eapply E.CTassign with (s:=s') (p:=q).
-      Focus 2. apply exp_trans_sound in H1. auto. admit.
+    - inversion H. subst. simpl in H14. inversion H14.
+      pose (equal_f H5 x).
+      unfold update in e0. rewrite <- beq_nat_refl in e0.
+      inversion e0. subst.
+      eapply E.CTassign with (s:=s') (p:=q); auto.
+      + eapply exp_trans_sound with (sG:=S.Cntxt vc lc) (t:=S.Typ s q). eauto.
+      + now destruct eG.
+  Qed.
   
 End TransProof.
